coq/Examples.v
@@ -1,0 +1,37 @@
+From Stdlib Require Import Utf8.
+Set Warnings "-notation-overridden,-parsing,-deprecated-hint-without-locality".
+From Stdlib Require Import Lia Strings.String Recdef Wf_nat Sorting.Permutation.
+From Stdlib.Lists Require Import List ListDec.
+Require Import Stdlib.Classes.Equivalence.
+Import ListNotations.
+
+From PolySimpl Require Import Syntax Utils VarList Algorithm BasicProps.
+From PolySimpl Require Import PFlattenProps ClearZPProps ReduceMonomProps ReconstructProps.
+From PolySimpl Require Import PolyUniqueness.
+
+Import Int.
+Open Scope string_scope.
+Open Scope Z_scope.
+Open Scope Int_scope.
+
+
+Eval compute in poly_simpl <{ X + X }>.
+Eval compute in poly_simpl <{ X - X }>.
+
+Eval compute in poly_simpl <{ 2*X - X }>.
+Eval compute in poly_simpl <{ Y - X }>.
+
+Eval compute in poly_simpl <{ 2*W*(X + 4*Y) - 13*(12*X*(7*W + X)+2*Y)+3*W}>.
+
+
+(* ======================================================================== *)
+(* new poly_simpl *)
+
+
+Eval compute in poly_simpl' <{ X + X }>.
+Eval compute in poly_simpl' <{ X - X }>.
+
+Eval compute in poly_simpl' <{ 2*X - X }>.
+Eval compute in poly_simpl' <{ Y - X }>.
+
+Eval compute in poly_simpl' <{ 2*W*(X + 4*Y) - 13*(12*X*(7*W + X)+2*Y)+3*W}>.
