coq/Maps.v
@@ -1,8 +1,8 @@
-From Coq Require Import Arith.Arith.
-From Coq Require Import Bool.Bool.
-Require Export Coq.Strings.String.
-From Coq Require Import Logic.FunctionalExtensionality.
-From Coq Require Import Lists.List.
+From Stdlib Require Import Arith.Arith.
+From Stdlib Require Import Bool.Bool.
+Require Export Stdlib.Strings.String.
+From Stdlib Require Import Logic.FunctionalExtensionality.
+From Stdlib Require Import Lists.List.
 Import ListNotations.
 Set Default Goal Selector "!".
 
