coq/ReconstructProps.v
@@ -1,6 +1,6 @@
-Require Import Utf8.
+From Stdlib Require Import Utf8.
 Set Warnings "-notation-overridden,-parsing,-deprecated-hint-without-locality".
-From Coq Require Import Lia Lists.List Strings.String Recdef Wf_nat.
+From Stdlib Require Import Lia Lists.List Strings.String Recdef Wf_nat.
 Import ListNotations.
 
 Require Import Syntax Utils BasicProps Algorithm.
@@ -42,5 +42,68 @@ Proof.
   simpl; subst.
   rewrite IHl', reconstruct_monom_correct.
   lia.
+Qed.
+
+
+(* ======================================================================== *)
+(* New reconstruct *)
+
+Lemma reconstruct_var_pow'_correct st x n :
+  aeval st (reconstruct_var_pow' x n) = (st x ^ Z.of_nat n)%Z.
+Proof.
+  Opaque Z.pow.
+  Opaque Z.of_nat.
+  induction n; auto; simpl;
+  remember (reconstruct_var_pow x n) as a'.
+  destruct n eqn:Ep; [ simpl; now rewrite <- Z.pow_1_r with (a:=st x) at 1 |].
+  assert (0 < n) by lia.
+  rewrite <- Ep in *; clear Ep n0.
+  cbn.
+  rewrite IHn; simpl.
+  replace (Z.of_nat (S n)) with (1 + Z.of_nat n)%Z by lia.
+  rewrite Z.pow_add_r; try lia.
+  Transparent Z.pow.
+  Transparent Z.of_nat.
+Qed.
+
+Lemma reconstruct_monom_fix'_correct st vs v :
+  aeval st (reconstruct_monom_fix' v vs) = fold_left Z.mul (map (pow st) (v::vs)) 1%Z.
+Proof.
+  revert v.
+  induction vs as [| [x n] l']; auto; simpl; intros [x' n']; autorewrite with zsimpl.
+  - (* now rewrite reconstruct_var_pow'_correct. *)
+    admit.
+  - simpl. rewrite IHl', <- fold_left_mul_acc.
+    (* now rewrite reconstruct_var_pow'_correct. *)
+    admit.
+Admitted.
+
+Lemma reconstruct_monom'_correct st c v :
+  aeval st (reconstruct_monom' c v) = fold_left Z.mul (map (pow st) v) c.
+Proof.
+  unfold reconstruct_monom'.
+  assert(aeval st
+    match v with
+    | [] => c
+    | v0 :: vs => <{ c * (reconstruct_monom_fix' v0 vs) }>
+    end = fold_left Z.mul (map (pow st) v) c). {
+    destruct v; auto.
+    rewrite fold_left_pull_acc, <- reconstruct_monom_fix'_correct; simpl; lia.
+    }
+  destruct c eqn:?; auto.
+  - destruct v; auto.
+  - destruct p eqn:?; auto.
+    destruct v; auto.
+    now rewrite <- reconstruct_monom_fix'_correct.
+Qed.
+
+
+Theorem reconstruct'_correct (p : pterm) (l : list pterm) :
+  reconstruct' p l ≲ₗ (p :: l).
+Proof.
+  intro st. revert p.
+  induction l as [| [c v] l']; auto; intros [c' v']; simpl.
+  - now rewrite reconstruct_monom'_correct.
+  - now rewrite IHl', reconstruct_monom'_correct.
 Qed.
 
